A state that can be compiled for posterity

FloatModel/Model/Float.lean
@@ -16,87 +16,87 @@ public import Init.Data.Order.Factories
 @[expose] public section
 
 /-- The logical model for the `Float` type. -/
-structure Float.Model where
+structure FloatModel.Model where
   /-- The underlying bit pattern of the `Float`. -/
   toBits : UInt64
   /-- The underlying bit pattern is valid according to the format. -/
-  valid : Float.Model.Format.binary64.Valid toBits.toBitVec
+  valid : FloatModel.Model.Format.binary64.Valid toBits.toBitVec
 
-namespace Float.Model
+namespace FloatModel.Model
 
-/-- Unpack a `Float.Model` into the corresponding `UnpackedFloat`. -/
-def unpack (f : Float.Model) : UnpackedFloat :=
+/-- Unpack a `FloatModel.Model` into the corresponding `UnpackedFloat`. -/
+def unpack (f : FloatModel.Model) : UnpackedFloat :=
   UnpackedFloat.unpack Format.binary64 f.toBits.toBitVec
 
 /--
-Pack an `UnpackedFloat` into the corresponding `Float.Model`.
+Pack an `UnpackedFloat` into the corresponding `FloatModel.Model`.
 This operation only gives a meaningful result if the float is
 already correctly rounded for the `Format.binary64` format.
 -/
-def pack (f : UnpackedFloat) : Float.Model where
+def pack (f : UnpackedFloat) : FloatModel.Model where
   toBits := UInt64.ofBitVec (UnpackedFloat.pack Format.binary64 f)
   valid := by simp
 
 /--
-Compute the sum of two `Float.Model`.
+Compute the sum of two `FloatModel.Model`.
 -/
-def add (a b : Float.Model) : Float.Model :=
+def add (a b : FloatModel.Model) : FloatModel.Model :=
   pack (UnpackedFloat.add Format.binary64 a.unpack b.unpack)
 
 /--
-Compute the difference of two `Float.Model`.
+Compute the difference of two `FloatModel.Model`.
 -/
-def sub (a b : Float.Model) : Float.Model :=
+def sub (a b : FloatModel.Model) : FloatModel.Model :=
   pack (UnpackedFloat.sub Format.binary64 a.unpack b.unpack)
 
 /--
-Compute the product of two `Float.Model`.
+Compute the product of two `FloatModel.Model`.
 -/
-def mul (a b : Float.Model) : Float.Model :=
+def mul (a b : FloatModel.Model) : FloatModel.Model :=
   pack (UnpackedFloat.mul Format.binary64 a.unpack b.unpack)
 
 /--
-Compute the quotient of two `Float.Model`.
+Compute the quotient of two `FloatModel.Model`.
 -/
-def div (a b : Float.Model) : Float.Model :=
+def div (a b : FloatModel.Model) : FloatModel.Model :=
   pack (UnpackedFloat.div Format.binary64 a.unpack b.unpack)
 
-instance : Add Float.Model where
+instance : Add FloatModel.Model where
   add a b := a.add b
 
-instance : Sub Float.Model where
+instance : Sub FloatModel.Model where
   sub a b := a.sub b
 
-instance : Mul Float.Model where
+instance : Mul FloatModel.Model where
   mul a b := a.mul b
 
-instance : Div Float.Model where
+instance : Div FloatModel.Model where
   div a b := a.div b
 
 /--
-Compute the square root of a `Float.Model`.
+Compute the square root of a `FloatModel.Model`.
 -/
-def sqrt (a : Float.Model) : Float.Model :=
+def sqrt (a : FloatModel.Model) : FloatModel.Model :=
   pack (UnpackedFloat.sqrt Format.binary64 a.unpack)
 
 /--
-Negate a `Float.Model`.
+Negate a `FloatModel.Model`.
 -/
-def neg (a : Float.Model) : Float.Model :=
+def neg (a : FloatModel.Model) : FloatModel.Model :=
   pack a.unpack.neg
 
 /--
-Return a `Float.Model` with positive sign.
+Return a `FloatModel.Model` with positive sign.
 -/
-def abs (a : Float.Model) : Float.Model :=
+def abs (a : FloatModel.Model) : FloatModel.Model :=
   pack a.unpack.abs
 
 /--
-Compute the ordering between two `Float.Model` as specified by IEEE. Returns an
+Compute the ordering between two `FloatModel.Model` as specified by IEEE. Returns an
 `Option Ordering` to account for the fact that `NaN` is incomparable with everything.
 Also, positive and negative zero are equal.
 -/
-protected def compare (a b : Float.Model) : Option Ordering :=
+protected def compare (a b : FloatModel.Model) : Option Ordering :=
   a.unpack.compare b.unpack
 
 /--
@@ -104,7 +104,7 @@ Determine whether `a` is less than or equal to `b` according to IEEE rules.
 
 This is not a total ordering, and `≤` is not reflexive.
 -/
-protected def le (a b : Float.Model) : Bool :=
+protected def le (a b : FloatModel.Model) : Bool :=
   a.unpack.le b.unpack
 
 /--
@@ -112,7 +112,7 @@ Determine whether `a` is less than `b` according to IEEE rules.
 
 This is not a total ordering.
 -/
-protected def lt (a b : Float.Model) : Bool :=
+protected def lt (a b : FloatModel.Model) : Bool :=
   a.unpack.lt b.unpack
 
 /--
@@ -120,131 +120,131 @@ Determine whether `a` is equal to `b` according to IEEE rules.
 
 This is not a reflexive relation.
 -/
-protected def beq (a b : Float.Model) : Bool :=
+protected def beq (a b : FloatModel.Model) : Bool :=
   a.unpack.beq b.unpack
 
-instance : LE Float.Model where
+instance : LE FloatModel.Model where
   le a b := a.le b
 
-instance : DecidableLE Float.Model :=
-  inferInstanceAs (∀ (a b : Float.Model), Decidable (a.le b))
+instance : DecidableLE FloatModel.Model :=
+  inferInstanceAs (∀ (a b : FloatModel.Model), Decidable (a.le b))
 
-instance : LT Float.Model where
+instance : LT FloatModel.Model where
   lt a b := a.lt b
 
-instance : DecidableLT Float.Model :=
-  inferInstanceAs (∀ (a b : Float.Model), Decidable (a.lt b))
+instance : DecidableLT FloatModel.Model :=
+  inferInstanceAs (∀ (a b : FloatModel.Model), Decidable (a.lt b))
 
-instance : BEq Float.Model where
+instance : BEq FloatModel.Model where
   beq a b := a.beq b
 
-instance : Min Float.Model :=
+instance : Min FloatModel.Model :=
   Min.leftLeaningOfLE _
 
-instance : Max Float.Model :=
+instance : Max FloatModel.Model :=
   Max.leftLeaningOfLE _
 
 /--
 Returns `true` if the float represents a real number, i.e., it is neither infinite nor `NaN`.
 -/
-def isFinite (a : Float.Model) : Bool :=
+def isFinite (a : FloatModel.Model) : Bool :=
   a.unpack.isFinite
 
 /--
 Returns `true` if the float is positive or negative infinity.
 -/
-def isInf (a : Float.Model) : Bool :=
+def isInf (a : FloatModel.Model) : Bool :=
   a.unpack.isInf
 
 /--
 Returns `true` if the float is `NaN`.
 -/
-def isNaN (a : Float.Model) : Bool :=
+def isNaN (a : FloatModel.Model) : Bool :=
   a.unpack.isNaN
 
 /--
-Construct a `Float.Model` from its bit representation. This operation canonicalizes
+Construct a `FloatModel.Model` from its bit representation. This operation canonicalizes
 all `NaN` inputs into the canonical `NaN`.
 -/
-def ofBits (a : UInt64) : Float.Model :=
+def ofBits (a : UInt64) : FloatModel.Model :=
   pack (UnpackedFloat.unpack Format.binary64 a.toBitVec)
 
-/-- Converts an `Int` to a `Float.Model`, returning positive zero on zero. -/
-def ofInt (n : Int) : Float.Model :=
+/-- Converts an `Int` to a `FloatModel.Model`, returning positive zero on zero. -/
+def ofInt (n : Int) : FloatModel.Model :=
   pack (UnpackedFloat.ofInt Format.binary64 n)
 
-/-- Converts a `Nat` to a `Float.Model`, returning positive zero on zero. -/
-def ofNat (n : Nat) : Float.Model :=
+/-- Converts a `Nat` to a `FloatModel.Model`, returning positive zero on zero. -/
+def ofNat (n : Nat) : FloatModel.Model :=
   pack (UnpackedFloat.ofNat Format.binary64 n)
 
-/-- Converts a `UInt8` to a `Float.Model`, returning positive zero on zero. -/
-def ofUInt8 (n : UInt8) : Float.Model :=
+/-- Converts a `UInt8` to a `FloatModel.Model`, returning positive zero on zero. -/
+def ofUInt8 (n : UInt8) : FloatModel.Model :=
   pack (UnpackedFloat.ofUInt8 Format.binary64 n)
 
-/-- Converts a `UInt16` to a `Float.Model`, returning positive zero on zero. -/
-def ofUInt16 (n : UInt16) : Float.Model :=
+/-- Converts a `UInt16` to a `FloatModel.Model`, returning positive zero on zero. -/
+def ofUInt16 (n : UInt16) : FloatModel.Model :=
   pack (UnpackedFloat.ofUInt16 Format.binary64 n)
 
-/-- Converts a `UInt32` to a `Float.Model`, returning positive zero on zero. -/
-def ofUInt32 (n : UInt32) : Float.Model :=
+/-- Converts a `UInt32` to a `FloatModel.Model`, returning positive zero on zero. -/
+def ofUInt32 (n : UInt32) : FloatModel.Model :=
   pack (UnpackedFloat.ofUInt32 Format.binary64 n)
 
-/-- Converts a `UInt64` to a `Float.Model`, returning positive zero on zero. -/
-def ofUInt64 (n : UInt64) : Float.Model :=
+/-- Converts a `UInt64` to a `FloatModel.Model`, returning positive zero on zero. -/
+def ofUInt64 (n : UInt64) : FloatModel.Model :=
   pack (UnpackedFloat.ofUInt64 Format.binary64 n)
 
-/-- Converts a `USize` to a `Float.Model`, returning positive zero on zero. -/
-def ofUSize (n : USize) : Float.Model :=
+/-- Converts a `USize` to a `FloatModel.Model`, returning positive zero on zero. -/
+def ofUSize (n : USize) : FloatModel.Model :=
   pack (UnpackedFloat.ofUSize Format.binary64 n)
 
-/-- Converts an `Int8` to a `Float.Model`, returning positive zero on zero. -/
-def ofInt8 (n : Int8) : Float.Model :=
+/-- Converts an `Int8` to a `FloatModel.Model`, returning positive zero on zero. -/
+def ofInt8 (n : Int8) : FloatModel.Model :=
   pack (UnpackedFloat.ofInt8 Format.binary64 n)
 
-/-- Converts an `Int16` to a `Float.Model`, returning positive zero on zero. -/
-def ofInt16 (n : Int16) : Float.Model :=
+/-- Converts an `Int16` to a `FloatModel.Model`, returning positive zero on zero. -/
+def ofInt16 (n : Int16) : FloatModel.Model :=
   pack (UnpackedFloat.ofInt16 Format.binary64 n)
 
-/-- Converts an `Int32` to a `Float.Model`, returning positive zero on zero. -/
-def ofInt32 (n : Int32) : Float.Model :=
+/-- Converts an `Int32` to a `FloatModel.Model`, returning positive zero on zero. -/
+def ofInt32 (n : Int32) : FloatModel.Model :=
   pack (UnpackedFloat.ofInt32 Format.binary64 n)
 
-/-- Converts an `Int64` to a `Float.Model`, returning positive zero on zero. -/
-def ofInt64 (n : Int64) : Float.Model :=
+/-- Converts an `Int64` to a `FloatModel.Model`, returning positive zero on zero. -/
+def ofInt64 (n : Int64) : FloatModel.Model :=
   pack (UnpackedFloat.ofInt64 Format.binary64 n)
 
-/-- Converts an `ISize` to a `Float.Model`, returning positive zero on zero. -/
-def ofISize (n : ISize) : Float.Model :=
+/-- Converts an `ISize` to a `FloatModel.Model`, returning positive zero on zero. -/
+def ofISize (n : ISize) : FloatModel.Model :=
   pack (UnpackedFloat.ofISize Format.binary64 n)
 
-/-- Converts a `Float.Model` to a `UInt8`. -/
-def toUInt8 (f : Float.Model) : UInt8 := f.unpack.toUInt8
+/-- Converts a `FloatModel.Model` to a `UInt8`. -/
+def toUInt8 (f : FloatModel.Model) : UInt8 := f.unpack.toUInt8
 
-/-- Converts a `Float.Model` to a `UInt16`. -/
-def toUInt16 (f : Float.Model) : UInt16 := f.unpack.toUInt16
+/-- Converts a `FloatModel.Model` to a `UInt16`. -/
+def toUInt16 (f : FloatModel.Model) : UInt16 := f.unpack.toUInt16
 
-/-- Converts a `Float.Model` to a `UInt32`. -/
-def toUInt32 (f : Float.Model) : UInt32 := f.unpack.toUInt32
+/-- Converts a `FloatModel.Model` to a `UInt32`. -/
+def toUInt32 (f : FloatModel.Model) : UInt32 := f.unpack.toUInt32
 
-/-- Converts a `Float.Model` to a `UInt64`. -/
-def toUInt64 (f : Float.Model) : UInt64 := f.unpack.toUInt64
+/-- Converts a `FloatModel.Model` to a `UInt64`. -/
+def toUInt64 (f : FloatModel.Model) : UInt64 := f.unpack.toUInt64
 
-/-- Converts a `Float.Model` to a `USize`. -/
-def toUSize (f : Float.Model) : USize := f.unpack.toUSize
+/-- Converts a `FloatModel.Model` to a `USize`. -/
+def toUSize (f : FloatModel.Model) : USize := f.unpack.toUSize
 
-/-- Converts a `Float.Model` to an `Int8`. -/
-def toInt8 (f : Float.Model) : Int8 := f.unpack.toInt8
+/-- Converts a `FloatModel.Model` to an `Int8`. -/
+def toInt8 (f : FloatModel.Model) : Int8 := f.unpack.toInt8
 
-/-- Converts a `Float.Model` to an `Int16`. -/
-def toInt16 (f : Float.Model) : Int16 := f.unpack.toInt16
+/-- Converts a `FloatModel.Model` to an `Int16`. -/
+def toInt16 (f : FloatModel.Model) : Int16 := f.unpack.toInt16
 
-/-- Converts a `Float.Model` to an `Int32`. -/
-def toInt32 (f : Float.Model) : Int32 := f.unpack.toInt32
+/-- Converts a `FloatModel.Model` to an `Int32`. -/
+def toInt32 (f : FloatModel.Model) : Int32 := f.unpack.toInt32
 
-/-- Converts a `Float.Model` to an `Int64`. -/
-def toInt64 (f : Float.Model) : Int64 := f.unpack.toInt64
+/-- Converts a `FloatModel.Model` to an `Int64`. -/
+def toInt64 (f : FloatModel.Model) : Int64 := f.unpack.toInt64
 
-/-- Converts a `Float.Model` to an `ISize`. -/
-def toISize (f : Float.Model) : ISize := f.unpack.toISize
+/-- Converts a `FloatModel.Model` to an `ISize`. -/
+def toISize (f : FloatModel.Model) : ISize := f.unpack.toISize
 
-end Float.Model
+end FloatModel.Model
